theories/AAC_hetero.v
@@ -23,7 +23,12 @@
    It handles assoc/commutaive functions over different types, but each function must be homogeneous (of shape X -> X -> X) *)
 
 Require Import Utils.
+Require Import BinPos.
 Require Export Interface.
+Require Import List.
+
+Local Open Scope list_scope.
+
 
 Set Implicit Arguments.
 Set Asymmetric Patterns.
@@ -34,22 +39,25 @@ Module ReifH.
     (* We use environments to store the various operators and the
      morphisms.*)
 
-    Variable e_type:idx -> Type.
+    Variable e_type: idx -> Type.
+
+    (* TODO: e_rel for different relations?*)
+    (*Variable e_rel : forall iTy, e_type iTy -> e_type iTy -> Prop.*)
 
     (** ** free symbols  *)
     Section Sym.
       (** type of an arity  *)
-      Fixpoint type_of_ar (ar: nelist idx) :=
-        match ar with
-        | nil i => e_type i
-        | cons i ar => (e_type i) -> type_of_ar ar
+      Fixpoint type_of_ar (args: list idx) ret:=
+        match args with
+        | nil => e_type ret
+        | i::args => (e_type i) -> type_of_ar args ret
         end.
 
       (** a symbol package contains an arity and a value of the corresponding type*)
-      Record Sym  : Type :=
+      Record Sym iTy: Type :=
         mkSym {
-            sym_ar : nelist idx;
-            sym_value :> type_of_ar sym_ar;
+            sym_args : list idx;
+            sym_value :> type_of_ar sym_args iTy;
           }.
 
     End Sym.
@@ -57,74 +65,67 @@ Module ReifH.
     (** ** binary operations *)
 
     Section Bin.
-      Record Bin :=
+      Record Bin iTy :=
         mkBin {
-            bin_iTy : idx;
-            bin_X := e_type bin_iTy;
-            bin_value:> bin_X -> bin_X -> bin_X;
-            bin_assoc: Associative (@eq bin_X) bin_value;
+            bin_value: e_type iTy -> e_type iTy -> e_type iTy;
+            bin_assoc: Associative eq bin_value;
             bin_comm: option (Commutative eq bin_value)
           }.
     End Bin.
 
     Arguments bin_value : clear implicits.
-    Arguments bin_iTy : clear implicits.
+    Arguments bin_value {iTy} _.
 
-    Variable e_sym: idx -> Sym.
-    Variable e_bin: idx -> Bin.
+    Variable e_sym: forall iTy, idx -> Sym iTy.
+    Variable e_bin: forall iTy, idx -> Bin iTy.
 
     (** packaging units (depends on e_bin) *)
 
     Record unit_of iTy (u:e_type iTy) :=
       mk_unit_for {
           uf_iBin: idx;
-          uf_bin := e_bin uf_iBin;
-          uf_eq : iTy = @bin_iTy uf_bin;
-          uf_desc: Unit (@eq _) (@bin_value uf_bin) (cast _ uf_eq u)
+          uf_bin := e_bin iTy uf_iBin;
+          uf_desc: Unit (@eq _) (bin_value uf_bin) u
         }.
 
 
-    Record unit_pack :=
+    Record unit_pack iTy :=
       mk_unit_pack {
-          u_iTy : idx;
-          u_value:> e_type u_iTy;
+          u_value:> e_type iTy;
           u_desc: list (unit_of u_value)
         }.
-    Variable e_unit: idx -> unit_pack.
+    Variable e_unit: forall iTy, idx -> unit_pack iTy.
 
     Inductive T: idx -> Type :=
-    | sum (i : idx) : let iTy := bin_iTy (e_bin i)
-                      in mset (T iTy) -> T iTy
+    | sum (iTy i : idx): mset (T iTy) -> T iTy
     (*| prd: idx -> nelist T -> T*)
-    | sym i: let ar := sym_ar (e_sym i) in
-             vT ar -> T (lastne ar)
-    | unit i: T (u_iTy (e_unit i))
-    with vT: nelist idx -> Type :=
-         | vnil X: vT (nil X)
+    | sym (iTy i : idx):
+             vT (sym_args (e_sym iTy i)) -> T iTy
+    | unit (iTy j:idx): T iTy
+    with vT: list idx -> Type :=
+         | vnil: vT nil
          | vcons X ar: T X -> vT ar -> vT (X::ar).
-
-    Arguments vnil {X}.
 
     (** lexicographic rpo over the normalised syntax *)
     Fixpoint compare {iTy jTy} (u: T iTy) (v: T jTy) :=
       match u,v with
-      | sum i l, sum j vs => lex (idx_compare i j) (mset_compare compare l vs)
+      | sum iTy i l, sum _ j vs => lex (idx_compare i j) (mset_compare compare l vs)
       (*| prd i l, prd j vs => lex (idx_compare i j) (list_compare compare l vs)*)
-      | sym i l, sym j vs => lex (idx_compare i j) (vcompare l vs)
-      | unit i , unit j => idx_compare i j
-      | unit _ , _        => Lt
-      | _      , unit _  => Gt
-      | sum _ _, _        => Lt
-      | _      , sum _ _  => Gt
+      | sym iTy i l, sym jTy j vs => lex (idx_compare i j) (vcompare l vs)
+      | unit _ i , unit _ j => (idx_compare i j)
+      | unit _ _ , _        => Lt
+      | _      , unit _ _  => Gt
+      | sum _ _ _, _        => Lt
+      | _      , sum _ _ _  => Gt
       (*| prd _ _, _        => Lt
       | _      , prd _ _  => Gt*)
 
       end
     with vcompare {ar1 ar2} (us: vT ar1) (vs: vT ar2) :=
            match us,vs with
-           | vnil _, vnil _ => Eq
-           | vnil _, _    => Lt
-           | _,    vnil _ => Gt
+           | vnil, vnil => Eq
+           | vnil, _  => Lt
+           | _,   vnil => Gt
            | vcons _ _ u us, vcons _ _ v vs => lex (compare u v) (vcompare us vs)
            end.
 
@@ -132,16 +133,604 @@ Module ReifH.
 
     Fixpoint eval {iTy} (u : T iTy) : (e_type iTy) :=
       match u with
-      | sum i l => let o := @bin_value (e_bin i) in
+      | sum iTy i l => let o := bin_value (e_bin iTy i) in
                   fold_map (fun un => let '(u,n):=un in @copy _ o n (eval u)) o l
       (*| prd i l => fold_map eval (Bin.value (e_bin i)) l*)
-      | sym i v => eval_aux v (sym_value (e_sym i))
-      | unit i  => e_unit i
+      | sym iTy i v => eval_aux v (sym_value (e_sym iTy i))
+      | unit iTy i  => e_unit iTy i
       end
-    with eval_aux {ar} (v: vT ar): type_of_ar ar -> e_type (lastne ar) :=
+    with eval_aux {ar iTy} (v: vT ar): type_of_ar ar iTy -> e_type iTy :=
            match v with
-           | vnil iTy => fun f => f
+           | vnil  => fun f => f
            | vcons X ar x v => fun f => eval_aux v (f (eval x))
            end.
 
+
+    (** we need to show that compare reflects equality (this is because
+     we work with msets rather than lists with arities) *)
+    Lemma tcompare_weak_spec: forall iTy (u v : T iTy), compare_weak_spec u v (compare u v)
+    with vcompare_reflect_eqdep: forall ar us ar' vs (H: ar=ar'), vcompare us vs = Eq -> cast vT H us = vs.
+    Proof.
+      -destruct u. 
+       +destruct v; simpl; try constructor.
+        case (pos_compare_weak_spec i i0); intros; try constructor.
+        case (mset_compare_weak_spec compare (tcompare_weak_spec iTy) m m0); intros; try constructor.
+       +intros u. destruct u. 1,3:now constructor. cbn.
+        destruct (pos_compare_weak_spec i i0); intros; try constructor.   
+        case_eq (vcompare v v0); intro Hv; try constructor.
+        rewrite <- (vcompare_reflect_eqdep _ _ _ _ eq_refl Hv). cbn. constructor.
+       +intros []. 1,2:now constructor. cbn.
+        case (pos_compare_weak_spec j j0); intros; try constructor. 
+      -induction us; destruct vs; simpl; intros H Huv; try discriminate.
+       +apply cast_eq, list_eq_dec, Pos.eq_dec.
+       +inversion H. subst.
+        revert Huv. case (tcompare_weak_spec _ t t0). 2,3:easy.
+        intro. intros H'. apply IHus with (H:=eq_refl) in H'. cbn in H'. subst.
+        apply cast_eq,list_eq_dec,Pos.eq_dec. 
+    Qed.
+    (*
+    Instance eval_aux_compat i (l: vT i): Proper (sym.rel_of X R i ==> R) (eval_aux l).
+    Proof.
+      induction l; simpl; repeat intro.
+      assumption.
+      apply IHl, H. reflexivity.
+    Qed.
+     *)
+    
+  (* in type iTy, is i a unit for [j] ? *)
+  Definition is_unit_of iTy j i :=
+    List.existsb (fun p => eq_idx_bool j (uf_iBin p)) (u_desc (e_unit iTy i)).
+
+  (* is [iTY i] commutative ? *)
+  Definition is_commutative iTy i :=
+    match bin_comm (e_bin iTy i) with Some _ => true | None => false end.
+
+
+  (** ** Normalisation *)
+
+  Inductive discr {A} : Type :=
+  | Is_op : A -> discr
+  | Is_unit : idx -> discr
+  | Is_nothing : discr .
+ 
+  (* This is called sum in the std lib *)
+  Inductive m {A} {B} :=
+  | left : A -> m
+  | right : B -> m.
+
+  (* combine intro rhs *)
+  Definition comp A B (merge : B -> B -> B) (l : B) (l' : @m A B) : @m A B :=
+    match l' with
+      | left _ => right l
+      | right l' => right (merge l l')
+    end.
+ 
+  (** auxiliary functions, to clean up sums  *)
+
+  Section sums.
+    Variable iTy : idx. (* index of the Type to look at *)
+    Variable i : idx. (* index of binary function to normalise *)
+    Variable is_unit : idx -> bool.
+
+
+    Definition sum' (u: mset (T iTy)): T iTy :=
+      match u with
+        | nilne (u,xH) => u
+        | _ => sum i u
+      end.
+
+    Definition is_sum  (u: T iTy) : @discr (mset (T iTy)) :=
+    match u with
+      | sum iTy j l => if eq_idx_bool j i then Is_op l else Is_nothing
+      | unit iTy j => if is_unit j   then Is_unit j else Is_nothing
+      | u => Is_nothing
+    end.
+
+    Definition copy_mset n (l: mset (T iTy)): mset (T iTy) :=
+      match n with
+        | xH => l
+        | _ => nelist_map (fun vm => let '(v,m):=vm in (v,Pmult n m)) l
+      end.
+   
+    Definition return_sum  u n :=
+      match is_sum  u with
+        | Is_nothing => right (nilne (u,n))
+        | Is_op l' =>  right (copy_mset n l')
+        | Is_unit j => left j
+      end.
+   
+    Definition add_to_sum u n (l : @m idx (mset (T iTy)))  :=
+      match is_sum  u with
+        | Is_nothing => comp (merge_msets compare) (nilne (u,n)) l
+        | Is_op l' => comp (merge_msets compare) (copy_mset n l') l
+        | Is_unit _ => l
+    end.
+
+
+    Definition norm_msets_ norm  (l: mset (T iTy)) :=
+    fold_map'
+    (fun un => let '(u,n) := un in  return_sum  (norm u) n)
+    (fun un l => let '(u,n) := un in  add_to_sum  (norm u) n l) l.
+
+
+  End sums.
+ 
+  (** similar functions for products *)
+
+  (* Section prds. *)
+
+  (*   Variable i : idx. *)
+  (*   Variable is_unit : idx -> bool. *)
+  (*   Definition prd'  (u: nelist T): T := *)
+  (*   match u with *)
+  (*     | nil u => u *)
+  (*     | _ => prd i u *)
+  (*   end. *)
+
+  (*   Definition is_prd (u: T) : @discr (nelist T) := *)
+  (*   match u with *)
+  (*     | prd j l => if eq_idx_bool j i then Is_op l else Is_nothing *)
+  (*     | unit j => if is_unit j  then Is_unit j else Is_nothing *)
+  (*     | u => Is_nothing *)
+  (*   end. *)
+ 
+   
+  (*   Definition return_prd u := *)
+  (*     match is_prd u with *)
+  (*       | Is_nothing => right (nil (u)) *)
+  (*       | Is_op l' =>  right (l') *)
+  (*       | Is_unit j => left j *)
+  (*     end. *)
+   
+  (*   Definition add_to_prd  u  (l : @m idx (nelist T))  := *)
+  (*     match is_prd  u with *)
+  (*       | Is_nothing => comp (@appne T) (nil (u)) l *)
+  (*       | Is_op l' => comp (@appne T) (l') l *)
+  (*       | Is_unit _ => l *)
+  (*     end. *)
+
+  (*   Definition norm_lists_ norm (l : nelist T) := *)
+  (*   fold_map' *)
+  (*   (fun u => return_prd  (norm u)) *)
+  (*   (fun u l => add_to_prd (norm u) l) l. *)
+
+
+  (* End prds. *)
+
+
+  (* Definition run_list x := match x with *)
+  (*                       | left n => nil (unit n) *)
+  (*                       | right l => l *)
+  (*                     end. *)
+ 
+  (* Definition norm_lists norm i l := *)
+  (*   let is_unit := is_unit_of i in *)
+  (*     run_list (norm_lists_ i is_unit norm l). *)
+
+  Definition run_msets {iTy} x := match x with
+                        | left n => nilne (unit iTy n, xH)
+                        | right l => l
+                      end.
+ 
+  Definition norm_msets {iTy} (norm: T iTy -> T iTy) i l :=
+    let is_unit := is_unit_of iTy i in
+      run_msets (norm_msets_ i is_unit norm l).
+ 
+  Fixpoint norm {iTy} (u:T iTy) {struct u} : T iTy:=
+    match u with
+      | sum iTy i l as u => if is_commutative iTy i then sum' i (norm_msets norm i l) else u
+      (* | prd i l => prd' i (norm_lists norm i l) *)
+      | sym iTy i l => sym iTy i (vnorm l)
+      | unit iTy i as u => u
+    end
+  with vnorm i (l: vT i): vT i :=
+    match l with
+      | vnil => vnil
+      | vcons _ _ u l => vcons (norm u) (vnorm l)
+    end.
+
+  (** ** Correctness *)
+
+  Lemma is_unit_of_Unit  : forall iTy i j : idx,
+   is_unit_of iTy i j = true -> Unit (@eq (e_type iTy)) (bin_value (e_bin iTy i)) (eval (unit iTy j)).
+  Proof.
+    intros. unfold is_unit_of in H.
+    rewrite existsb_exists in H.
+    destruct H as [x [H H']].
+    revert H' ; case (eq_idx_spec); [intros H' _ ; subst| intros _ H'; discriminate].
+    simpl. destruct x. simpl. auto.
+  Qed.
+ 
+  Instance Binvalue_Commutative iTy i (H : is_commutative iTy i = true) : Commutative eq (bin_value (e_bin iTy i) ).
+  Proof.
+    unfold is_commutative in H.
+    destruct bin_comm; auto.
+    discriminate.
+  Qed.
+
+  Instance Binvalue_Associative iTy i :Associative eq (bin_value (e_bin iTy i) ).
+  Proof.
+    destruct e_bin; auto.
+  Qed.
+ (*
+  Instance Binvalue_Proper i : Proper (R ==> R ==> R) (@Bin.value _ _ (e_bin i) ).
+  Proof.
+    destruct ((e_bin i)); auto.
+  Qed.
+*)
+  Hint Resolve (*Binvalue_Proper*) Binvalue_Associative Binvalue_Commutative.
+
+  (** auxiliary lemmas about sums  *)
+
+  Hint Resolve is_unit_of_Unit.
+  Section sum_correctness.
+    Variable iTy i : idx. (* The binary operator of the sum*)
+    Variable is_unit : idx -> bool.
+    Hypothesis is_unit_sum_Unit : forall j, is_unit j = true -> @Unit _ eq (bin_value (e_bin iTy i)) (eval (unit iTy j)).
+
+    Inductive is_sum_spec_ind iTy: T iTy -> @discr (mset (T iTy)) -> Prop :=
+    | is_sum_spec_op : forall j l, j = i -> is_sum_spec_ind (sum j l) (Is_op l)
+    | is_sum_spec_unit : forall j, is_unit j = true ->  is_sum_spec_ind (unit iTy j) (Is_unit j)
+    | is_sum_spec_nothing : forall u, is_sum_spec_ind u (Is_nothing).
+ 
+    Lemma is_sum_spec (u:T iTy) : is_sum_spec_ind u (is_sum i is_unit u).
+    Proof.
+      unfold is_sum; destruct u; intros; try constructor.
+      -destruct eq_idx_bool eqn:eq1. 2: now constructor.
+      revert eq1. case eq_idx_spec; try discriminate. intros. now  constructor.
+      -case_eq (is_unit j); intros; try constructor. auto.
+    Qed.
+
+    Instance assoc :   @Associative _ eq (bin_value (e_bin iTy i)).
+    Proof.
+      destruct (e_bin iTy i). simpl. assumption.
+    Qed.
+    (*Instance proper :   Proper (R ==> R ==> R) (Bin.value (e_bin i)).
+    Proof.
+      destruct (e_bin i). simpl. assumption.
+    Qed.*)
+    Hypothesis comm : @Commutative _ eq (bin_value (e_bin iTy i)).
+
+    Lemma sum'_sum : forall  (l: mset (T iTy)),  eval (sum' i l) = eval (sum i l) .
+    Proof.
+      intros [[a n] | [a n] l]; destruct n;  simpl; reflexivity.
+    Qed.
+
+    Lemma eval_sum_nil (x:T iTy):
+      eval (sum i (nilne (x,xH))) = (eval x).
+    Proof. rewrite <- sum'_sum. reflexivity.   Qed.
+     
+    Lemma eval_sum_cons : forall n a (l: mset (T iTy)),
+      (eval (sum i ((a,n):::l))) = (bin_value (e_bin iTy i) (@copy _ (bin_value (e_bin iTy i)) n (eval a)) (eval (sum i l))).
+    Proof.
+      intros n a [[? ? ]|[b m] l]; simpl; reflexivity.
+    Qed.
+   
+    Inductive compat_sum_unit : @m idx (mset (T iTy)) -> Prop :=
+    | csu_left : forall x,  is_unit x = true->  compat_sum_unit  (left x)
+    | csu_right : forall m, compat_sum_unit (right m).
+
+    Lemma compat_sum_unit_return x n : compat_sum_unit  (return_sum i is_unit x n).
+    Proof.
+      unfold return_sum.
+      case is_sum_spec; intros; try constructor; auto.
+    Qed.
+   
+    Lemma compat_sum_unit_add : forall x n h,
+        compat_sum_unit  h ->
+        compat_sum_unit
+          (add_to_sum i (is_unit_of iTy i) x n
+                      h).
+    Proof.
+      unfold add_to_sum;intros; inversion H;
+        case_eq  (is_sum i (is_unit_of iTy i) x);
+        intros; simpl; try constructor || eauto. apply H0.
+    Qed.
+
+    (* Hint Resolve copy_plus. : this lags because of  the inference of the implicit arguments *)
+    Hint Extern 5 (copy (?n + ?m) (eval ?a) = bin_value (copy ?n (eval ?a)) (copy ?m (eval ?a))) => apply copy_plus.
+    Hint Extern 5 (?x = ?x) => reflexivity.
+    Hint Extern 5 (bin_value ?x ?y = bin_value ?y ?x) => apply bin_comm.
+   
+    Lemma eval_merge_bin : forall (h k: mset (T iTy)),
+      eval (sum i (merge_msets compare h k)) = bin_value (e_bin iTy i) (eval (sum i h)) (eval (sum i k)).
+    Proof.
+      induction h as [[a n]|[a n] h IHh]; intro k.
+      -simpl.
+       induction k as [[b m]|[b m] k IHk]; simpl.
+       +destruct (tcompare_weak_spec a b) as [a|a b|a b]; simpl; auto. apply copy_plus; auto.  all: exact _. 
+     
+       +destruct (tcompare_weak_spec a b) as [a|a b|a b]; simpl; auto.
+        rewrite copy_plus,law_assoc; auto. now cbv;congruence. 
+        rewrite IHk;  clear IHk. rewrite 2 law_assoc. f_equal. apply law_comm.
+        
+      -induction k as [[b m]|[b m] k IHk]; simpl;  simpl in IHh.
+      +destruct (tcompare_weak_spec a b) as [a|a b|a b]; simpl.
+       *rewrite  (law_comm _ (copy m (eval a))), law_assoc, <- copy_plus,  Pplus_comm; auto. now cbv;congruence. 
+       *rewrite <- law_assoc, IHh.  reflexivity.
+       *rewrite law_comm. reflexivity.
+      +simpl in IHk.
+       destruct (tcompare_weak_spec a b) as [a|a b|a b]; simpl.
+       *rewrite IHh; clear IHh. rewrite 2 law_assoc. rewrite (law_comm _ (copy m (eval a))). rewrite law_assoc, <- copy_plus,  Pplus_comm; auto. cbv;congruence. 
+       *rewrite IHh; clear IHh. simpl.  rewrite law_assoc. reflexivity. 
+       *rewrite 2 (law_comm  (copy m (eval b))). rewrite law_assoc.  
+       rewrite <- IHk. reflexivity.
+    Qed.
+
+ 
+    Lemma copy_mset' n (l: mset (T iTy)):  copy_mset n l = nelist_map (fun vm => let '(v,m):=vm in (v,Pmult n m)) l.
+    Proof.
+      unfold copy_mset.  destruct n; try reflexivity.
+     
+      simpl. induction l as [|[a l] IHl]; simpl; try congruence.  destruct a.  reflexivity.
+    Qed.
+   
+   
+    Lemma copy_mset_succ  n (l: mset (T iTy)):  eval (sum i (copy_mset (Pos.succ n) l)) = bin_value (e_bin iTy i) (eval (sum i l)) (eval (sum i (copy_mset n l))).
+    Proof.
+      rewrite 2 copy_mset'.
+     
+      induction l as [[a m]|[a m] l IHl].
+      -simpl eval.   rewrite <- copy_plus; auto. rewrite Pmult_Sn_m. reflexivity. cbv. congruence. 
+      -simpl nelist_map.  rewrite ! eval_sum_cons. rewrite IHl.  clear IHl.
+       rewrite Pmult_Sn_m. rewrite copy_plus; auto. rewrite <- !law_assoc. 2:now cbv;congruence.
+       f_equal. 
+       rewrite law_comm . rewrite <- !law_assoc. f_equal. apply law_comm.
+    Qed.
+
+    Lemma copy_mset_copy : forall n  (m : mset (T iTy)), eval (sum i (copy_mset n m)) = @copy _ (bin_value (e_bin iTy i)) n (eval (sum i m)).
+    Proof.
+      induction n using Pind; intros.
+     
+      unfold copy_mset. rewrite copy_xH. reflexivity.
+      rewrite copy_mset_succ. rewrite copy_Psucc. rewrite IHn. reflexivity.
+    Qed.
+   
+    Instance compat_sum_unit_Unit : forall p, compat_sum_unit (left p) ->
+      @Unit _ eq (bin_value (e_bin iTy i)) (eval (unit iTy p)).
+    Proof.
+      intros.
+      inversion H. subst.  auto.
+    Qed.
+  
+    Lemma copy_n_unit : forall j n, is_unit j = true ->
+      eval (unit iTy j) = @copy _ (bin_value (e_bin iTy i)) n (eval (unit iTy j)).
+    Proof.
+      intros.
+      induction n using Prect.
+      rewrite copy_xH. reflexivity.
+      rewrite copy_Psucc. rewrite <- IHn. apply is_unit_sum_Unit in H. rewrite law_neutral_left. reflexivity.
+    Qed.
+
+   
+    Lemma z0  l r (H : compat_sum_unit  r):
+      eval (sum i (run_msets (comp (merge_msets compare) l r))) = eval (sum i ((merge_msets compare) (l) (run_msets r))).
+    Proof.
+      unfold comp. unfold run_msets.
+      case_eq r; intros; subst.
+      rewrite eval_merge_bin; auto.
+      rewrite eval_sum_nil.
+      apply compat_sum_unit_Unit in H. rewrite law_neutral_right.  reflexivity.
+      reflexivity.
+    Qed.
+
+    Lemma z1 : forall n x,
+      eval (sum i (run_msets (return_sum i (is_unit) x n )))
+      = @copy _ (bin_value (e_bin iTy i)) n (eval x).
+    Proof.
+      intros. unfold return_sum.  unfold run_msets.
+      destruct (is_sum_spec x); intros; subst.
+      -rewrite copy_mset_copy.
+       reflexivity.
+      -rewrite eval_sum_nil. apply copy_n_unit. auto.
+      -reflexivity.
+    Qed.
+    Lemma z2 : forall  u n x, compat_sum_unit  x ->
+      eval (sum i ( run_msets
+        (add_to_sum i (is_unit) u n x)))
+      = 
+      bin_value (e_bin iTy i) (@copy _ (bin_value (e_bin iTy i))  n (eval u)) (eval (sum i (run_msets x))).
+    Proof.
+      intros u n x Hix .
+      unfold add_to_sum.
+      case is_sum_spec; intros; subst.
+   
+      rewrite z0 by auto.  rewrite eval_merge_bin.  rewrite copy_mset_copy. reflexivity.
+      rewrite <- copy_n_unit by assumption.
+      apply is_unit_sum_Unit in H.
+      rewrite law_neutral_left. reflexivity.
+     
+     
+      rewrite z0 by auto.  rewrite eval_merge_bin. reflexivity.
+    Qed.
+  End sum_correctness.
+  
+  Lemma eval_norm_msets iTy i norm
+    (Comm : Commutative eq (bin_value (e_bin iTy i)))
+    (Hnorm: forall (u : T iTy), eval (norm u) = eval u) : forall h, eval (sum i (norm_msets norm i h)) = eval (sum i h).
+  Proof.
+    unfold norm_msets.
+    assert (H :
+      forall h : mset (T iTy),
+        eval (sum i (run_msets (norm_msets_ i (is_unit_of iTy i) norm h))) =  eval (sum i h) /\ compat_sum_unit (is_unit_of iTy i) (norm_msets_ i (is_unit_of iTy i) norm h)).
+      
+    -induction h as [[a n] | [a n] h [IHh IHh']]; simpl norm_msets_; split.
+     +rewrite z1 by auto.  rewrite Hnorm . reflexivity.
+     +apply compat_sum_unit_return. auto.      
+     +rewrite z2 by auto. rewrite IHh. 
+      rewrite eval_sum_cons.  rewrite Hnorm. reflexivity.
+     +apply compat_sum_unit_add, IHh'.
+     -apply H.
+  Defined.
+ 
+  (** auxiliary lemmas about products  *)
+
+  (* Section prd_correctness. *)
+  (*   Variable iTy i : idx. *)
+  (*   Variable is_unit : idx -> bool. *)
+  (*   Hypothesis is_unit_prd_Unit : forall j, is_unit j = true->  @Unit _ eq (bin_value (e_bin iTy i)) (eval (unit j)). *)
+
+  (*   Inductive is_prd_spec_ind  : T ->  @discr (nelist T) -> Prop := *)
+  (*   | is_prd_spec_op : *)
+  (*     forall j l, j = i -> is_prd_spec_ind (prd j l) (Is_op l) *)
+  (*   | is_prd_spec_unit : *)
+  (*     forall j, is_unit j = true ->  is_prd_spec_ind (unit j) (Is_unit j) *)
+  (*   | is_prd_spec_nothing : *)
+  (*     forall u, is_prd_spec_ind u (Is_nothing). *)
+   
+  (*   Lemma is_prd_spec u : is_prd_spec_ind u (is_prd i is_unit u). *)
+  (*   Proof. *)
+  (*     unfold is_prd; case u; intros; try constructor. *)
+  (*     case (eq_idx_spec); intros; subst;  try constructor; auto. *)
+  (*     case_eq (is_unit p); intros; try constructor; auto.   *)
+  (*   Qed. *)
+
+  (*   Lemma prd'_prd : forall (l: nelist T), eval (prd' i l) == eval (prd i l). *)
+  (*   Proof. *)
+  (*     intros  [?|? [|? ?]]; simpl; reflexivity. *)
+  (*   Qed. *)
+   
+   
+  (*   Lemma eval_prd_nil x:  eval (prd i (nil x)) == eval x.  *)
+  (*   Proof. *)
+  (*     rewrite <- prd'_prd. simpl. reflexivity. *)
+  (*   Qed. *)
+  (*   Lemma eval_prd_cons a : forall (l: nelist T), eval (prd i (a::l)) == @Bin.value _ _ (e_bin i) (eval a) (eval (prd i l)). *)
+  (*   Proof. *)
+  (*     intros  [|b l]; simpl; reflexivity. *)
+  (*   Qed.        *)
+  (*   Lemma eval_prd_app : forall (h k: nelist T), eval (prd i (h++k)) == @Bin.value _ _ (e_bin i) (eval (prd i h)) (eval (prd i k)). *)
+  (*   Proof. *)
+  (*     induction h; intro k. simpl; try reflexivity. *)
+  (*     simpl appne.  rewrite  2 eval_prd_cons, IHh, law_assoc. reflexivity. *)
+  (*   Qed.        *)
+
+  (*   Inductive compat_prd_unit : @m idx (nelist T) -> Prop := *)
+  (*   | cpu_left : forall x,  is_unit  x = true -> compat_prd_unit  (left x) *)
+  (*   | cpu_right : forall m, compat_prd_unit (right m) *)
+  (*   . *)
+ 
+  (*   Lemma compat_prd_unit_return  x: compat_prd_unit (return_prd i is_unit x). *)
+  (*   Proof. *)
+  (*     unfold return_prd. *)
+  (*     case (is_prd_spec); intros; try constructor; auto. *)
+  (*   Qed. *)
+
+  (*   Lemma compat_prd_unit_add  : forall x  h, *)
+  (*     compat_prd_unit  h *)
+  (*     -> *)
+  (*     compat_prd_unit *)
+  (*     (add_to_prd i is_unit x *)
+  (*       h). *)
+  (*   Proof. *)
+  (*     intros. *)
+  (*     unfold add_to_prd. *)
+  (*     unfold comp. *)
+  (*     case (is_prd_spec); intros; try constructor; auto. *)
+  (*     unfold comp; case h; try constructor. *)
+  (*     unfold comp; case h; try constructor. *)
+  (*   Qed. *)
+
+   
+  (*   Instance compat_prd_Unit : forall p, compat_prd_unit (left p) -> *)
+  (*     @Unit X R (Bin.value (e_bin i)) (eval (unit p)). *)
+  (*   Proof. *)
+  (*     intros. *)
+  (*     inversion H; subst. apply is_unit_prd_Unit. assumption. *)
+  (*   Qed. *)
+
+  (*   Lemma z0' : forall l (r: @m idx (nelist T)), compat_prd_unit r -> *)
+  (*     eval (prd i (run_list (comp (@appne T) l r))) == eval (prd i ((appne (l) (run_list r)))). *)
+  (*   Proof. *)
+  (*     intros. *)
+  (*     unfold comp. unfold run_list. case_eq r; intros; auto; subst. *)
+  (*     rewrite eval_prd_app. *)
+  (*     rewrite eval_prd_nil. *)
+  (*     apply compat_prd_Unit in H. rewrite law_neutral_right. reflexivity. *)
+  (*     reflexivity. *)
+  (*   Qed. *)
+ 
+  (*   Lemma z1' a :  eval (prd i (run_list (return_prd i is_unit a))) ==  eval (prd i (nil a)). *)
+  (*   Proof. *)
+  (*     intros. unfold return_prd.  unfold run_list. *)
+  (*     case (is_prd_spec); intros; subst; reflexivity. *)
+  (*   Qed. *)
+  (*   Lemma z2' : forall  u  x, compat_prd_unit  x ->  *)
+  (*     eval (prd i ( run_list *)
+  (*       (add_to_prd i is_unit u x))) ==  @Bin.value _ _ (e_bin i) (eval u) (eval (prd i (run_list x))). *)
+  (*   Proof. *)
+  (*     intros u x Hix. *)
+  (*     unfold add_to_prd. *)
+  (*     case (is_prd_spec); intros; subst. *)
+  (*     rewrite z0' by auto.  rewrite eval_prd_app.  reflexivity. *)
+  (*     apply is_unit_prd_Unit in H. rewrite law_neutral_left. reflexivity. *)
+  (*     rewrite z0' by auto.  rewrite eval_prd_app. reflexivity. *)
+  (*   Qed. *)
+ 
+  (* End prd_correctness. *)
+
+
+
+
+  (* Lemma eval_norm_lists i (Hnorm: forall u, eval (norm u) = eval u) : forall h, eval (prd i (norm_lists norm i h)) = eval (prd i h). *)
+  (* Proof. *)
+  (*   unfold norm_lists. *)
+  (*   assert (H :  forall h : nelist T, *)
+  (*     eval (prd i (run_list (norm_lists_ i (is_unit_of i) norm h))) == *)
+  (*     eval (prd i h) *)
+  (*     /\ compat_prd_unit (is_unit_of i) (norm_lists_ i (is_unit_of i) norm h)). *)
+  
+   
+  (*     induction h as [a | a h [IHh IHh']]; simpl norm_lists_; split. *)
+  (*     rewrite z1'. simpl.  apply Hnorm. *)
+   
+  (*     apply compat_prd_unit_return. *)
+   
+  (*     rewrite z2'. rewrite IHh.  rewrite eval_prd_cons.  rewrite Hnorm. reflexivity. apply is_unit_of_Unit. *)
+  (*     auto. *)
+
+  (*     apply compat_prd_unit_add. auto. *)
+  (*     apply H. *)
+  (*   Defined. *)
+
+  (** correctness of the normalisation function *)
+
+  Theorem eval_norm: forall iTy (u: T iTy), eval (norm u) = eval u
+    with eval_norm_aux: forall arTy ret (l: vT arTy) (f: type_of_ar arTy ret),
+      eval_aux (vnorm l) f = eval_aux l f.
+  Proof.
+    induction u as [ iTy p m (*| iTY p l*) | iTy ? | iTy ?];  cbn [norm].
+    -case_eq (is_commutative iTy p); intros.
+     +rewrite sum'_sum.
+      apply eval_norm_msets; auto.
+     +reflexivity.
+    (*-rewrite prd'_prd.
+    apply eval_norm_lists; auto.*)
+    -apply eval_norm_aux.
+    -reflexivity.
+    -induction l; cbn; intros f.
+     +reflexivity.
+     +rewrite eval_norm. apply IHl; reflexivity.
+  Qed.
+
+
+  (** corollaries, for goal normalisation or decision *)
+
+  Lemma normalise : forall iTy (u v: T iTy), eval (norm u) = eval (norm v) -> eval u = eval v.
+  Proof. intros ? u v. rewrite 2 eval_norm. trivial. Qed.
+   
+  Lemma compare_reflect_eq iTy (u v : T iTy) : compare u v = Eq -> eval u = eval v.
+  Proof. case (tcompare_weak_spec u v); intros; try congruence. Qed.
+
+  Lemma decide iTy (u v: T iTy): compare (norm u) (norm v) = Eq -> eval u = eval v.
+  Proof. intros H. apply normalise. apply compare_reflect_eq. apply H. Qed.
+
+  (* Lemma lift_normalise {S} {H : AAC_lift S R}: *)
+  (*   forall (u v: T), (let x := norm u in let y := norm v in *)
+  (*     S (eval x) (eval y)) -> S (eval u) (eval v). *)
+  (* Proof. destruct H. intros u v; simpl; rewrite 2 eval_norm. trivial. Qed. *)
+
+
   End ReifH.
+End ReifH.
+
